Foundation/Modal/Kripke/Hilbert/KTc.lean
@@ -1,0 +1,31 @@
+import Foundation.Modal.Kripke.Hilbert.Geach
+
+namespace LO.Modal
+
+open Kripke
+open Geachean
+
+abbrev Kripke.CoreflexiveFrameClass : FrameClass := { F | Coreflexive F }
+
+namespace Hilbert.KTc
+
+instance Kripke.sound : Sound (Hilbert.KTc) (Kripke.CoreflexiveFrameClass) := by
+  convert Hilbert.Geach.Kripke.sound (G := {⟨0, 1, 0, 0⟩});
+  exact eq_Geach;
+  . unfold CoreflexiveFrameClass MultiGeacheanConfluentFrameClass MultiGeachean;
+    simp [Geachean.reflexive_def, Geachean.coreflexive_def];
+
+instance Kripke.consistent : Entailment.Consistent (Hilbert.KTc) := by
+  convert Hilbert.Geach.Kripke.Consistent (G := {⟨0, 1, 0, 0⟩});
+  exact eq_Geach;
+
+instance Kripke.complete : Complete (Hilbert.KTc) (Kripke.CoreflexiveFrameClass) := by
+  convert Hilbert.Geach.Kripke.Complete (G := {⟨0, 1, 0, 0⟩});
+  . exact eq_Geach;
+  . unfold CoreflexiveFrameClass MultiGeacheanConfluentFrameClass MultiGeachean;
+    simp [Geachean.coreflexive_def];
+
+end Hilbert.KTc
+
+
+end LO.Modal
